improving explore; explore_have: have/if/for structure

lib/Explorer.thy
@@ -8,7 +8,7 @@
 
 theory Explorer
 imports Main
-keywords "explore" :: diag
+keywords "explore" "explore_have" :: diag
 begin
 
 subsection {* Explore command *}
@@ -21,17 +21,29 @@ fun split_clause t =
     val shows = Logic.strip_imp_concl horn;
   in (fixes, assms, shows) end;
 
-fun isar_skeleton ctxt (fixes, assms, shows) =
+fun space_implode_with_line_break l =
+  if length l > 1 then
+     "\n    " ^ space_implode  " and\n    " l
+  else
+    space_implode  " and\n    " l
+
+fun isar_skeleton ctxt is_have (fixes, assms, shows) =
   let
+    val kw_fix = if is_have then "  for " else "  fix "
+    val kw_assume = if is_have then "  if " else "  assume "
+    val kw_goal = if is_have then "  have " else "  show "
     val fixes_s = if null fixes then NONE
-      else SOME ("fix " ^ space_implode " and "
+      else SOME (kw_fix ^ space_implode " and "
         (map (fn (v, T) => v ^ " :: " ^ quote (Syntax.string_of_typ ctxt T)) fixes));
     val (_, ctxt') = Variable.add_fixes (map fst fixes) ctxt; 
     val assumes_s = if null assms then NONE
-      else SOME ("assume " ^ space_implode " and "
+      else SOME (kw_assume ^ space_implode_with_line_break
         (map (quote o Syntax.string_of_term ctxt') assms))
-    val shows_s = ("show " ^ (quote o Syntax.string_of_term ctxt') shows ^ " sorry")
-    val s = cat_lines (map_filter I [fixes_s, assumes_s] @ [shows_s]);
+    val shows_s = (kw_goal ^ (quote o Syntax.string_of_term ctxt') shows)
+    val s = 
+      if is_have
+      then cat_lines (shows_s :: map_filter I [assumes_s, fixes_s] @ ["  sorry"])
+      else cat_lines (map_filter I [fixes_s, assumes_s] @ [shows_s ^ " sorry"]);
   in
     s
   end;
@@ -42,7 +54,7 @@ fun explore st =
     val goal_props = Logic.strip_imp_prems (Thm.prop_of goal);
     val clauses = map split_clause goal_props;
     val text = cat_lines
-      ("proof -" :: separate "next" (map (isar_skeleton context) clauses) @ ["qed"]);
+      ("proof -" :: separate "next" (map (isar_skeleton context false) clauses) @ ["qed"]);
     val message = Active.sendback_markup_properties [] text;
   in
     (st |> tap (fn _ => Output.information message))
@@ -56,6 +68,26 @@ val _ =
     "explore current goal state as Isar proof"
     (Scan.succeed explore_cmd)
 
+fun explore_have st =
+  let
+    val { context, facts = _, goal } = Proof.goal st;
+    val goal_props = Logic.strip_imp_prems (Thm.prop_of goal);
+    val clauses = map split_clause goal_props;
+    val text = cat_lines
+      (separate "" (map (isar_skeleton context true) clauses));
+    val message = Active.sendback_markup_properties [] text;
+  in
+    (st |> tap (fn _ => Output.information message))
+  end
+
+
+val explore_have_cmd =
+  Toplevel.keep_proof (K () o explore_have o Toplevel.proof_of)
+
+val _ =
+  Outer_Syntax.command @{command_keyword "explore_have"}
+    "explore current goal state as Isar proof with have, if and for"
+    (Scan.succeed explore_have_cmd)
 *}
 
 subsection {* Examples *}
@@ -66,6 +98,7 @@ lemma
   apply simp_all
   apply auto
   explore
-    oops
+  explore_have
+  oops
 
 end
